src/PlutusIR/Semantics/Static/normaliser_STLC/gu_naive/TypeReductionSOP.v
@@ -4,19 +4,6 @@ Require Import Coq.Strings.String.
 
 Require Import Coq.Lists.List.
 
-Inductive Empty : Type :=.
-
-Definition Not {A B : Type} (P : A -> B -> Type) (x : A) (y : B) : Type :=
-  P x y -> Empty.
-
-Inductive ExactlyOneSetPair {A B : Type} (P : A -> B -> Type) : list A -> list B -> Type :=
-  | ExactlyOneSP_head : forall x y xs ys,
-      P x y ->
-      ForallSetPair (Not P)  xs ys ->
-      ExactlyOneSetPair P (x :: xs) (y :: ys)
-  | ExactlyOneSP_tail : forall x y xs ys,
-      Not P x y -> ExactlyOneSetPair P xs ys -> ExactlyOneSetPair P (x :: xs) (y :: ys).
-
 (* Deterministic step function for PlutusIR type system *)
 Inductive step : ty -> ty -> Type :=
     | step_beta (X : string) (K : kind) (S T : ty) :
@@ -42,9 +29,12 @@ Inductive step : ty -> ty -> Type :=
     | step_ifixR F T1 T2 :
         normal_Ty F ->
         step T1 T2 -> step (Ty_IFix F T1) (Ty_IFix F T2)
-    | step_SOP Tss_normal Tss1 Tss2 Tss_remainder :
-        ForallSet normal_Ty Tss_normal ->  (* Tss_normal can be empty, so this allows all reductions*)
-        step Tss1 Tss2 ->
-        step (Ty_SOP (Tss_normal ++ Tss1 :: Tss_remainder)) (Ty_SOP (Tss_normal ++ Tss2 :: Tss_remainder))
+    | step_SOP Tss_normal Tss_sub_normal Tss_sub1 Tss_sub2 Tss_sub_remainder Tss_remainder :
+        (* List of list of types, we can reduce if only one of them steps, and everything "before" it is normal *)
+        ForallSet2 normal_Ty Tss_normal ->  (* Tss_normal can be empty, so this allows all reductions*)
+        ForallSet normal_Ty Tss_sub_normal -> (* The inner list should also have normal types before the type that is stepping*)
+        step Tss_sub1 Tss_sub2 ->
+        step (Ty_SOP (Tss_normal ++ (Tss_sub_normal ++ Tss_sub1 :: Tss_sub_remainder) :: Tss_remainder)) 
+             (Ty_SOP (Tss_normal ++ (Tss_sub_normal ++ Tss_sub2 :: Tss_sub_remainder) :: Tss_remainder))
     .
     
